Veir/IR/OpInfo.lean
@@ -1,0 +1,36 @@
+module
+
+namespace Veir
+
+public section
+
+/--
+The `HasOpInfo` type class provides information about opcodes and their properties
+and how to hash, represent, and compare them for equality. It also
+provides a type family `propertyOf` that maps an operation code to the type of
+its properties
+-/
+class HasOpInfo (opCode: Type)
+    extends Hashable opCode, Repr opCode, Inhabited opCode where
+  propertiesOf : opCode → Type
+  propertiesHash {op : opCode} : Hashable (propertiesOf op)
+  propertiesDefault {op : opCode} : Inhabited (propertiesOf op)
+  propertiesRepr {op : opCode} : Repr (propertiesOf op)
+  propertiesDecideEq {op : opCode} : DecidableEq (propertiesOf op)
+  decideEq : DecidableEq (opCode)
+
+instance [HasOpInfo opCode] {op : opCode} : Hashable (HasOpInfo.propertiesOf op) where
+  hash := HasOpInfo.propertiesHash.hash
+
+instance [HasOpInfo opCode] {op : opCode} : Inhabited (HasOpInfo.propertiesOf op) where
+  default := HasOpInfo.propertiesDefault.default
+
+instance [HasOpInfo opCode] {op : opCode} : Repr (HasOpInfo.propertiesOf op) where
+  reprPrec := HasOpInfo.propertiesRepr.reprPrec
+
+instance [HasOpInfo opCode] : DecidableEq (opCode) :=
+  HasOpInfo.decideEq
+
+end -- public section
+
+end Veir
